{
\fontsize{10}{10}\selectfont
$$
\int_0^1 t^{x-1}(1-t)^{y-1}\,dt = \mathrm{beta}(x,y) = \frac{\Gamma(x)\Gamma(y)}{\Gamma(x+y)}
$$

$$
\int_0^{+\infty} t^{num-1}e^{-t}\,dt = \mathrm{tgamma}(num) = e^{\mathrm{lgamma}(num)}
$$

$$
\int_0^{phi} \frac{d\theta}{\sqrt{1-k^2\sin^2\theta}} = \mathrm{ellint\_1}(k,phi)
$$

$$
\int_0^{phi} \sqrt{1-k^2\sin^2\theta}\,d\theta = \mathrm{ellint\_2}(k,phi)
$$

$$
\int_{num}^{+\infty} \frac{e^{-t}}{t}\,dt = -\mathrm{expint}(-num)
$$

$$
\sum_{n=1}^{+\infty} n^{-num} = \mathrm{riemann\_zeta}(num)
$$

$$
\frac{2}{\sqrt{\pi}}\int_0^{arg} e^{-t^2}\,dt = \mathrm{erf}(arg)
$$

%$$
%J_{\alpha} (x) = \sum_{m = 0}^{\infty} \frac{(-1)^m}{m ! \Gamma (m + \alpha + 1)} \left(\frac{x}{2}\right) ^ {(2 m + \alpha)} = \mathrm{jn} (\alpha, x)
%$$
%
%$$
%Y_{\alpha} (x) = \frac{J_{\alpha} (x) \cos (\alpha \pi) - J_{ - \alpha} (x)}{\sin (\alpha \pi)} = \mathrm{yn} (\alpha, x)
%$$
}
