$$
d(i \cdot j) = \sum_{p \mid i, p \mid j} \mu (p) \cdot d (\frac{i}{p}) \cdot d (\frac{j}{p})
\qquad
\epsilon (x) = \sum \limits_{d \mid x} \mu (d)
$$

$$
\mathrm{I} * \mathrm{I} = \mathrm{d}
\quad
\mathrm{\varphi} * \mathrm{I} = \mathrm{Id}
\quad
\Lambda * \mathrm{I} = \log
\quad
\mathrm{Id}_k * \mathrm{I} = \mathrm{\sigma}_k
\quad
\mathrm{\mu} * \mathrm{I} = \mathrm{\epsilon}
$$

$$
f * g = h \implies g(1) * S(n) = \sum_{i = 1}^{n} h(i) - \sum_{i = 2}^{n} g(i) S(\left \lfloor \frac{n}{i} \right \rfloor)
$$

$$
f = g * h \implies h(p ^ c) = f(p ^ c) - \sum_{i = 1}^{c} g(p ^ i) \cdot h(p ^ {c-i})
$$
